src/Bedrock/Specs/Field.v
@@ -22,7 +22,6 @@ Class FieldParameters :=
     mul : string; add : string; sub : string; opp : string;
     square : string; scmula24 : string; inv : string;
     from_bytes : string; to_bytes : string;
-    from_mont : string; to_mont : string; (*only for word-by-word Montgomery*)
     select_znz : string;
 
     (* felem_small_literal p x :=
@@ -48,14 +47,6 @@ Class FieldRepresentation
        :=
   { felem := list word;
     feval : felem -> F M_pos;
-    (*  
-        TODO: do we actually need this?
-        feval_alt is used only by word-by-word Montgomery,
-        as it needs to distinguish between evaulation with/without
-        pulling the argument out of Montgomery domain.
-        For Solinas, this is the same as feval
-    *)
-    feval_alt : felem -> F M_pos; 
 
     feval_bytes : list byte -> F M_pos;
     felem_size_in_words : nat;
@@ -222,7 +213,7 @@ Section FunctionSpecs.
         /\ (FElem pout out * Rr)%sep mem;
       ensures tr' mem' :=
         tr = tr' /\
-        exists X, feval_alt X = feval_bytes bs
+        exists X, feval X = feval_bytes bs
              /\ bounded_by tight_bounds X
              /\ (FElem pout X * Rr)%sep mem' }.
 
@@ -234,7 +225,7 @@ Section FunctionSpecs.
         /\ (FElemBytes pout out * Rr)%sep mem;
       ensures tr' mem' :=
         tr = tr'
-        /\ let bs := Z_to_bytes (F.to_Z (feval_alt x))
+        /\ let bs := Z_to_bytes (F.to_Z (feval x))
                                 encoded_felem_size_in_bytes in
            (FElemBytes pout bs * Rr)%sep mem' }.
 
@@ -262,10 +253,6 @@ Section FunctionSpecs.
     fnspec! select_znz (pout pc px py : word) / out Rout Rx Ry x y,
     {
         requires tr mem :=
-        (*Are this list_Z_bounded_by's necessary? Can this information be inferred from FElem?*)
-        list_Z_bounded_by (@max_bounds width felem_size_in_words) (List.map word.unsigned x) /\
-        list_Z_bounded_by (@max_bounds width felem_size_in_words) (List.map word.unsigned y) /\
-        list_Z_bounded_by (@max_bounds width felem_size_in_words) (List.map word.unsigned out) /\
         (FElem pout out * Rout)%sep mem /\
         (FElem px x * Rx)%sep mem /\
         (FElem py y * Ry)%sep mem /\
@@ -284,10 +271,10 @@ Section FunctionSpecs.
     Definition from_mont_model x := F.mul x (@F.of_Z M_pos (r' ^ (Z.of_nat felem_size_in_words)%Z)).
     Definition to_mont_model x := F.mul x (@F.of_Z M_pos (r ^ (Z.of_nat felem_size_in_words)%Z)).
   
-    Instance un_from_mont : UnOp from_mont :=
+    Instance un_from_mont {from_mont : string} : UnOp from_mont :=
       {| un_model := from_mont_model; un_xbounds := tight_bounds; un_outbounds := loose_bounds |}.
   
-    Instance un_to_mont : UnOp to_mont :=
+    Instance un_to_mont {to_mont : string} : UnOp to_mont :=
       {| un_model := to_mont_model; un_xbounds := tight_bounds; un_outbounds := loose_bounds|}.
 
 End FunctionSpecs.
