src/COperationSpecifications.v
@@ -195,15 +195,6 @@ Module selectznz.
     Local Notation eval := (Positional.eval wt n).
 
     Definition selectznz_correct
-               (selectznz : Z -> list Z -> list Z -> list Z)
-      := forall cond x y,
-        is_bounded_by0 r[0~>1] cond = true
-        -> list_Z_bounded_by saturated_bounds x
-        -> list_Z_bounded_by saturated_bounds y
-        -> eval (selectznz cond x y) = (if Decidable.dec (cond = 0) then eval x else eval y)
-           /\ list_Z_bounded_by saturated_bounds (selectznz cond x y).
-
-    Definition selectznz_correct_alt
         (selectznz : Z -> list Z -> list Z -> list Z)
       := forall cond x y,
       is_bounded_by0 r[0~>1] cond = true
@@ -625,18 +616,9 @@ Module WordByWordMontgomery.
            /\ valid (from_bytes x).
 
     Definition selectznz_correct
-               (selectznz : Z -> list Z -> list Z -> list Z)
-      : Prop
-      := selectznz.selectznz_correct
-           (UniformWeight.uweight bitwidth)
-           n
-           saturated_bounds
-           selectznz.
-
-    Definition selectznz_correct_alt
                 (selectznz : Z -> list Z -> list Z -> list Z)
       : Prop
-      := selectznz.selectznz_correct_alt
+      := selectznz.selectznz_correct
             saturated_bounds
             selectznz.
 
