src/PushButtonSynthesis/Primitives.v
@@ -858,7 +858,7 @@ Section __.
           machine_wordsize prefix "selectznz" selectznz
           (docstring_with_summary_from_lemma!
              (fun fname : string => [text_before_function_name ++ fname ++ " is a multi-limb conditional select."]%string)
-             (selectznz_correct dummy_weight n saturated_bounds)).
+             (selectznz_correct saturated_bounds)).
   Definition mulx (s : Z)
     := Pipeline.BoundsPipeline
          false (* subst01 *)
@@ -1045,10 +1045,10 @@ Section __.
   Lemma Wf_cmovznz_by_mul s' res (Hres : cmovznz_by_mul s' = Success res) : Wf res.
   Proof using Type. prove_pipeline_wf (). Qed.
 
-  Lemma selectznz_correct limbwidth res
+  Lemma selectznz_correct res
         (Hres : selectznz = Success res)
-    : selectznz_correct (weight (Qnum limbwidth) (QDen limbwidth)) n saturated_bounds (Interp res).
-  Proof using Type. prove_correctness I. Qed.
+    : selectznz_correct saturated_bounds (Interp res).
+  Proof using Type. prove_correctness I. eapply select_eq; eauto. Qed.
 
   Lemma Wf_selectznz res (Hres : selectznz = Success res) : Wf res.
   Proof using Type. prove_pipeline_wf (). Qed.
